End of day 21/03/18

michael_formal/types.thy
@@ -3,27 +3,39 @@ theory types
 begin
 type_synonym label = string
 type_synonym arity = nat
-type_synonym inputs = "int list"
+type_synonym inputs = state
 type_synonym registers = state
-type_synonym outputs = "int list"
-type_synonym guard = "inputs \<Rightarrow> registers \<Rightarrow> bool"
-type_synonym output_function = "inputs \<Rightarrow> registers \<Rightarrow> outputs"
-type_synonym update_function = "inputs \<Rightarrow> registers \<Rightarrow> registers"
+type_synonym outputs = state
+type_synonym guard = "bexp list"
+type_synonym output_function = "(string \<times> aexp) list"
+type_synonym update_function = "(string \<times> aexp) list"
 type_synonym statename = int
-type_synonym trace = "(label \<times>(int list)) list" (*Ideally written as label(i1, i2, ...)*)
+type_synonym trace = "(label \<times> state) list" (*Ideally written as label(i1, i2, ...)*)
 type_synonym observation = "outputs list"
 
+
 record transition = 
-  Label :: "label"
-  Arity :: "arity"
-  Guard :: "guard"
-  Outputs :: "output_function"
-  Updates :: "update_function"
+  Label :: label
+  Arity :: arity
+  Guard :: guard
+  Outputs :: output_function
+  Updates :: update_function
 
 type_synonym destination = "(statename \<times> transition)"
 
 record efsm =
   S :: "statename list"
-  s0 :: "statename"
-  T :: "(statename * statename) \<Rightarrow> transition list"
+  s0 :: statename
+  T :: "(statename \<times> statename) \<Rightarrow> transition list"
+
+definition join :: "state \<Rightarrow> state \<Rightarrow> state" where
+  "join s1 s2 = (\<lambda>x. if (aval (V x) s1) \<noteq> 0 then (aval (V x) s1) else (aval (V x) s2))"
+declare join_def [simp]
+
+lemma "\<forall>z. \<exists>x y. (aval (V v) (join x y) = aval (V v) z)"
+  by auto
+
+lemma "\<forall> x y. \<exists>z. (aval (V v) z) = aval (V v) (join x y)"
+  by auto
+
 end
